theories/zoo_parabs/future__opaque.v
@@ -1,6 +1,7 @@
 From zoo_parabs Require Import
   future__code.
 
+#[global] Opaque future_return.
 #[global] Opaque future_async.
 #[global] Opaque future_wait.
 #[global] Opaque future_iter.
